Let us consider orthogonal vectors $\vec{m}_1$ and $\vec{m}_2$ to the given
normal vector $\vec{n}$. Let $\vec{m} = \myvec{a\\ b\\ c}$.

Then, 
\begin{align}
	\vec{m}^T\vec{n} = 0 \\
	\implies \quad \myvec{a & b & c}\myvec{2\\ 3\\-4} = 0   \label{eq:solutions/4/45/1/2/mTn} \\
	\implies \quad 2a + 3b -4c = 0 
\end{align}
Let $a=1$, \ $b=0$, so that
\begin{align}
	\vec{m}_1 = \myvec{1 \\ 0 \\ \frac{1}{2}} 
\end{align}
and $a=0$, \ $b=1$, so that
\begin{align}
	\vec{m}_2 = \myvec{0 \\ 1 \\ \frac{3}{4}} 
\end{align}
We, now, solve the equation
\begin{align}
	\vec{M}\vec{x} = \vec{b} 	\label{eq:solutions/4/45/1/2/matrixeq}
\end{align}
which, upon substitution, becomes
\begin{align}
\myvec{1 & 0\\ 0 & 1 \\ \frac{1}{2} & \frac{3}{4}}\vec{x}=\myvec{3 \\ -2 \\ 0} 
\end{align}
	Any $m\times n$ matrix $\vec{M}$ can be factorized in SVD form as
\begin{align}
	\vec{M} = \vec{U}\vec{S}\vec{V}^T	\label{eq:solutions/4/45/1/2/svd}
\end{align}
where $\vec{U}$ and $\vec{V}$ are matrices of eigen vectors which are orthogonal. Columns of $\vec{V}$ are the eigen vectors of $\vec{M}^T\vec{M}$,columns of $\vec{U}$ are the eigen vectors of $\vec{M}\vec{M}^T$ and $\vec{S}$ is the diagonal matrix of singular values of $\vec{M}$ of the eigenvalues of $\vec{M}^T\vec{M}$.
\begin{align}
	\vec{M}^T\vec{M} = 
	\myvec{\frac{10}{8} & \frac{3}{8} \\ \frac{3}{8} & \frac{25}{16} }
\end{align}
Putting (\ref{eq:solutions/4/45/1/2/svd}) into (\ref{eq:solutions/4/45/1/2/matrixeq}), we get
\begin{align}
	\vec{U}\vec{S} \vec{V}^T\vec{x} = \vec{b} \\
    \implies \qquad \vec{x} = \vec{V}\vec{S}_{+}\vec{U}^T\vec{b} \label{eq:solutions/4/45/1/2/calcx}
\end{align}
where \ $\vec{S}_{+}$ is the Moore-Penrose Pseudoinverse of $\vec{S}$.

The eigenvalues of $\vec{M}^T\vec{M}$:
\begin{align}
	\mydet{\vec{M}^T\vec{M}-\lambda \vec{I}} = 0 \\
	\implies \quad
	\mydet{\frac{10}{8}-\lambda & \frac{3}{8} \\ \frac{3}{8} & \frac{25}{16}-\lambda } = 0 \\
	\implies \quad
	\lambda^2 - \frac{45}{16}\lambda + \frac{116}{64} = 0
\end{align}
	So, the eigenvalues are 
\begin{align}
	\lambda_1 = \frac{29}{16}	\\
	\lambda_2 = 1
\end{align}
For $\lambda_1 = \frac{29}{16}$, the eigen vector $\vec{v_1}$ can be calculated using row reduction as :
\begin{align}
	\myvec{-\frac{9}{16} & \frac{3}{8} \\ \frac{3}{8} & -\frac{4}{16}} 
	\xleftrightarrow[]{R_1 \leftarrow - \frac{16}{9}R_1}
	\myvec{1 & -\frac{2}{3} \\ \frac{3}{8} & -\frac{4}{16}} \\
	\xleftrightarrow[]{R_2 \leftarrow R_2-R_1}
	\myvec{1 & -\frac{2}{3} \\ 0 & 0} 
\end{align}
Hence, 
\begin{align}
	\vec{v_1}= \myvec{\frac{2}{\sqrt{13}} \\ \frac{3}{\sqrt{13}}}
\end{align}
Similarly, for $\lambda_2=1$, 
\begin{align}
	\vec{v_2}= \myvec{-\frac{3}{\sqrt{13}} \\ \frac{2}{\sqrt{13}}}
\end{align}
Thus, 
\begin{align}
	\vec{V}= \myvec{\frac{2}{\sqrt{13}} & -\frac{3}{\sqrt{13}} \\
		\frac{3}{\sqrt{13}} & \frac{2}{\sqrt{13}} }
\end{align}
Now, 
\begin{align}
	\vec{M}\vec{M}^T = 
	\myvec{1 & 0 & \frac{1}{2} \\ 0 & 1 & \frac{3}{4} \\
		\frac{1}{2} & \frac{3}{4} & \frac{13}{16} }
\end{align}
Now, calculating eigenvalues of $\vec{M}\vec{M}^T$
\begin{align}
	\mydet{1-\lambda & 0 & \frac{1}{2} \\ 0 & 1-\lambda & \frac{3}{4} \\
		\frac{1}{2} & \frac{3}{4} & \frac{13}{16}-\lambda } = 0  
\end{align}
	So, the eigenvalues are 
\begin{align}
	\lambda_1 = \frac{29}{16}	\\
	\lambda_2 = 1	\\
	\lambda_3 = 0
\end{align}
For $\lambda_1 = \frac{29}{16}$, the eigen vector can be computed as:
\begin{align}
	\myvec{1-\frac{29}{16} & 0 & \frac{1}{2} \\
	 0 & 1 - \frac{29}{16} & \frac{3}{4} \\
	\frac{1}{2} & \frac{3}{4} & \frac{13}{16}-\frac{29}{16} }  \\
	\xleftrightarrow[]{}
	\myvec{-\frac{13}{16} & 0 & \frac{1}{2}\\ 
	0 & -\frac{13}{16} & \frac{3}{4} \\
	\frac{1}{2} & \frac{3}{4} & -1} \\
	\xleftrightarrow[]{R_1 \leftarrow - \frac{16}{13}R_1}
	\myvec{1 & 0 & -\frac{8}{3} \\ 0 & -\frac{13}{16} & \frac{3}{4} \\
	\frac{1}{2} & \frac{3}{4} & -1} \\
	\xleftrightarrow[]{R_3 \leftarrow R_3-\frac{1}{2}R_1}
	\myvec{1 & 0 & -\frac{8}{3} \\ 0 & -\frac{13}{16} & \frac{3}{4} \\
	0 & \frac{3}{4} & -\frac{9}{13} } \\
	\xleftrightarrow[]{R_2 \leftarrow -\frac{16}{13}R_2}
	\myvec{1 & 0 & -\frac{8}{3} \\ 0 & 1 & -\frac{12}{13} \\
	0 & \frac{3}{4} & -\frac{9}{13} } 
\end{align}
\begin{align}
	\xleftrightarrow[]{R_2 \leftarrow R_3-\frac{3}{4}R_2}
	\myvec{1 & 0 & -\frac{8}{3} \\ 0 & 1 & -\frac{12}{13} \\
	0 & 0 & 0 }
\end{align}
Hence, the eigen vector $\vec{u}_1$:
\begin{align}
	\vec{u_1}= \myvec{\frac{8}{\sqrt{377}} \\ \frac{12}{\sqrt{377}} \\
	\frac{13}{\sqrt{377}} }
\end{align}
For $\lambda_2=1$, the eigen vector is:
\begin{align}
	\myvec{1-1 & 0 & \frac{1}{2} \\ 0 & 1-1 & \frac{3}{4} \\
	\frac{1}{2} & \frac{3}{4} & \frac{13}{16}-1 }  \\
	\xleftrightarrow[]{}
	\myvec{0 & 0 & \frac{1}{2} \\ 0 & 0 & \frac{3}{4} \\
	\frac{1}{2} & \frac{3}{4} & -\frac{3}{16} }  
\end{align}
Hence, the eigen vector $\vec{u}_2$:
\begin{align}
	\vec{u_2}= \myvec{\frac{3}{\sqrt{13}} \\ -\frac{2}{\sqrt{13}} \\ 0 }
\end{align}
Similarly, for $\lambda_3=0$, the eigen vector is:
\begin{align}
	\myvec{1 & 0 & \frac{1}{2} \\ 0 & 1 & \frac{3}{4} \\
	\frac{1}{2} & \frac{3}{4} & \frac{13}{16} }  \\
	\xleftrightarrow[]{R_3 \leftarrow R_3-\frac{1}{2}R_1-\frac{3}{4}R_2}
	\myvec{0 & 0 & \frac{1}{2} \\ 0 & 0 & \frac{3}{4} \\
	0	& 	0	&	0 } 
\end{align}
Hence, the eigen vector $\vec{u}_3$:
\begin{align}
	\vec{u_3}= \myvec{\frac{2}{\sqrt{29}} \\ \frac{3}{\sqrt{29}} \\ 
	-\frac{4}{\sqrt{29}} }
\end{align}
So, the orthonormal matrix $\vec{U}$ of eigen vectors is:
\begin{align}
   \vec{U}= \myvec{
	   \frac{8}{\sqrt{377}} & \frac{3}{\sqrt{13}} & \frac{2}{\sqrt{29}}  \\ 
	   \frac{12}{\sqrt{377}} & -\frac{2}{\sqrt{13}} & \frac{3}{\sqrt{29}}\\ 
	   \frac{13}{\sqrt{377}} & 0 & -\frac{4}{\sqrt{29}} }
\end{align}
The matrix of singular values of $\vec{M}$ is: 
\begin{align}
   \vec{S}= \myvec{ \frac{\sqrt{29}}{4} & 0 & 0 \\
	   0 & 1 & 0 \\ 0 & 0 & 0}
\end{align}
The Moore-Penrose pseudoinverse of $\vec{S}$ is computed as
\begin{align}
	\vec{S}_{+} &= (\vec{S}\vec{S}^T)^{-1}\vec{S}^T 	\\
		&= \myvec{ \frac{4}{\sqrt{29}} & 0 & 0 \\ 0 & 1 & 0 }
\end{align}
To solve for $\vec{x}$ in (\ref{eq:solutions/4/45/1/2/calcx}), noting that $\vec{b}=\myvec{3 \\ -2 \\ 0}$, 
\begin{align}
\vec{U}^T\vec{b} = \myvec{
	0 \\ \sqrt{13} \\ 0 } \\
\vec{S}_{+}\vec{U}^T\vec{b} = \myvec{ 0 \\ \sqrt{13} }
\end{align}
Thus, the foot of perpendicular is:
\begin{align}
\vec{x} = \vec{V}\vec{S}_{+}\vec{U}^T\vec{b} 
	&= \myvec{\frac{2}{\sqrt{13}} & -\frac{3}{\sqrt{13}} \\
		\frac{3}{\sqrt{13}} & \frac{2}{\sqrt{13}} }
	  \myvec{ 0 \\ \sqrt{13} }
	\\
	\implies \quad
\vec{x} &= \myvec{ -3 \\ 2 }  	\label{eq:solutions/4/45/1/2/xeq}
\end{align}

The solution can be verified using
\begin{align}
	\vec{M}^T\vec{M}\vec{x} = \vec{M}^T\vec{b}
\end{align}
The LHS gives
\begin{align}
	& \vec{M}^T\vec{M}\vec{x} 
	= \myvec{\frac{10}{8} & \frac{3}{8} \\ \frac{3}{8} & \frac{25}{16} }
	\myvec{-3 \\ 2} \\
	\implies
	& \vec{M}^T\vec{M}\vec{x} = \myvec{-3 \\ 2} 
\end{align}
Now, finding $\vec{x}$ from 
\begin{align}
	\myvec{\frac{10}{8} & \frac{3}{8} \\ \frac{3}{8} & \frac{25}{16} }
	\vec{x} = \myvec{-3 \\ 2} 
\end{align}
Solving the augmented matrix, we get
\begin{align}
     \myvec{\frac{10}{8} & \frac{3}{8} & -3 \\ \frac{3}{8} & \frac{25}{16} & 2}
	\xleftrightarrow[]{R_1 \leftarrow -\frac{3}{10}R_1}
     \myvec{1 & \frac{3}{10} &-\frac{24}{10} \\ \frac{3}{8} & \frac{25}{16} & 2}
	\\
	\xleftrightarrow[]{R_2 \leftarrow R_2-\frac{3}{8}R_1}
	\myvec{1 & \frac{3}{10} &-\frac{24}{10} \\ 
		0 & \frac{29}{20} & \frac{58}{20} }
	\xleftrightarrow[]{R_2 \leftarrow \frac{20}{29}R_2} \myvec{1 & \frac{3}{10} &-\frac{24}{10} \\ 0 & 1 & 2 } \\
	\xleftrightarrow[]{R_1 \leftarrow R_1-\frac{3}{10}R_2}
	\myvec{1 & 0 & -3 \\ 0 & 1 & 2}
\end{align}
Hence, the solution is given by
\begin{align}
	\vec{x} = \myvec{ -3 \\ 2 } 	\label{eq:solutions/4/45/1/2/xverifyeq}
\end{align}
Comparing the results in Eq.(\ref{eq:solutions/4/45/1/2/xeq}) and (\ref{eq:solutions/4/45/1/2/xverifyeq}), it is
concluded that the solution is verified.

