Equation of plane can be written in the form: 
\begin{align}\label{eq:solutions/4/44/1/d/eq1}
	\vec{n}^T\vec{x} &= c
\end{align}
Writing the given plane equation \eqref{eq:solutions/4/44/1/d/eq:1.0.1} in the form \eqref{eq:solutions/4/44/1/d/eq1}:
\begin{align}\label{eq:solutions/4/44/1/d/eq2}
	\myvec{3 & 2 & -6}\myvec{x\\y\\z} &= 2
\intertext{Where,}
    \vec{n} &= \myvec{3\\2\\-6} \\
    \vec{x} &= \myvec{x\\y\\z}  \quad  c = 2
\end{align}
A vector from the plane to the point $D(-1, 2, -4)$ is given by:
\begin{align}
\vec{w}=\vec{d}-\vec{x}
\intertext{Where,}
    \vec{d} &= \myvec{-1\\2\\-4} \\
    \vec{x} &= \myvec{x\\y\\z} 
\end{align}
The projection of $\vec{w}$ onto the normal vector $\vec{n}$ can be written as:
\begin{align}
    \text{proj}_\vec{n}\vec{w}=\frac{\vec{n}^T\vec{w}}{\vec{n}^T\vec{n}}\cdot\vec{n}\\
    \text{proj}_\vec{n}\vec{w}=\frac{\vec{n}^T(\vec{d}-\vec{x})}{\vec{n}^T\vec{n}}\cdot\vec{n}\\
     \text{proj}_\vec{n}\vec{w}=\frac{\vec{n}^T\vec{d}-\vec{n}^T\vec{x}}{\vec{n}^T\vec{n}}\cdot\vec{n}\\
\end{align}
From equation \eqref{eq:solutions/4/44/1/d/eq1},
\begin{align}
     \text{proj}_\vec{n}\vec{w}=\frac{\vec{n}^T\vec{d}-c}{\vec{n}^T\vec{n}}\cdot\vec{n}\\
\end{align}
Putting the values of $\vec{n}$, $\vec{d}$ and $c$, we get:
\begin{align}
     \text{proj}_\vec{n}\vec{w}=\frac{\myvec{3&2&-6}\myvec{-1\\2\\-4} -2}{\myvec{3&2&-6}\myvec{3\\2\\-6}}\cdot\myvec{3\\2\\-6}\\
      \text{proj}_\vec{n}\vec{w}=\frac{23}{49}\cdot\myvec{3\\2\\-6}
\end{align}
The distance $d_{min}$ between point $D(-1, 2, -4)$ and the given plane  is obtained as:
\begin{align}
    d_{min}=\norm{\text{proj}_\vec{n}\vec{w}}\\
    d_{min}=\frac{23}{49}\cdot\norm{\myvec{3\\2\\-6}}
\end{align}
\begin{align}
    \therefore d_{min}=\frac{23}{49} \times \sqrt{(3)^2+(2)^2+(-6)^2}\\
    \therefore d_{min}=\frac{23}{49} \times 7\\
    \implies \boxed{d_{min}=\frac{23}{7}= 3.2857} \label{eq:solutions/4/44/1/d/eq_20}
\end{align}
%\begin{figure}[h!]
%\centering
%\resizebox{\columnwidth}{!}
%    {
%    \input{Figure.tex}
%    }
%    \caption{Distance between a point and a plane}
%\end{figure}
%\\
\textbf{Finding the foot of perpendicular from point $\vec{D}$ to the given plane using SVD:}\\
We need to represent the equation of plane in parametric form,
\begin{align}
	\vec{Q} = \vec{p} + \alpha_1\vec{m_1} + \alpha_2\vec{m_2}\label{eq:solutions/4/44/1/d/eq3}
\end{align}
Here $\vec{p}$ is any point on plane and $\vec{m_1}, \vec{m_2}$ are two vectors parallel to plane and hence $\perp$ to $\vec{n}$.
First we find orthogonal vectors $\vec{m_1}$ and $\vec{m_2}$ to the vector $\vec{n}$. Let, $\vec{m} = \myvec{a\\b\\c}$, then
\begin{align}
\vec{m^T}\vec{n} &= 0 \nonumber \\
\implies \myvec{a & b & c} \myvec{3 \\ 2 \\ -6} &= 0 \nonumber \\
\implies 3a+2b-6c &= 0 \label{eq:solutions/4/44/1/d/eq:eq_1}
\end{align}
By substituting $a=1;b=0$ in \eqref{eq:solutions/4/44/1/d/eq:eq_1},
\begin{align} \label{eq:solutions/4/44/1/d/eq:eq_2}
    \vec{m_1} = \myvec{1 \\ 0 \\ 1/2} 
\end{align}
By substituting $a=0;b=1$ in \eqref{eq:solutions/4/44/1/d/eq:eq_1},
\begin{align} \label{eq:solutions/4/44/1/d/eq:eq_3}
    \vec{m_2} = \myvec{0 \\ 1 \\ 1/3} 
\end{align}
Let us find point $\vec{p}$ on the plane. Put $x=1,z=0$ in \eqref{eq:solutions/4/44/1/d/eq2}, we get $\vec{p} = \myvec{1\\\frac{-1}{2}\\0}$\\
Let $\vec{Q}$ be the point on plane with shortest distance to point $\vec{d}$.
$\vec{Q}$ can be expressed in \eqref{eq:solutions/4/44/1/d/eq3} form as
\begin{align}\label{eq:solutions/4/44/1/d/eq6}
	\vec{Q} = \myvec{1\\\frac{-1}{2}\\0} + \alpha_1\myvec{1\\0\\\frac{1}{2}} + \alpha_2\myvec{0\\1\\\frac{1}{3}} \label{eq:solutions/4/44/1/d/eq_25}
\end{align}
Computation of Pseudo Inverse using SVD in order to determine the value of $\alpha_1$ and $\alpha_2$ :
\begin{align}
	\label{eq:solutions/4/44/1/d/eq7}\myvec{1\\\frac{-1}{2}\\0} + \alpha_1\myvec{1\\0\\\frac{1}{2}} + \alpha_2\myvec{0\\1\\\frac{1}{3}} &= \myvec{-1\\2\\-4}\\\label{eq:solutions/4/44/1/d/eq8}
	\alpha_1\myvec{1\\0\\\frac{1}{2}} + \alpha_2\myvec{0\\1\\\frac{1}{3}}  &= \myvec{-2\\\frac{5}{2}\\-4}\\\label{eq:solutions/4/44/1/d/eq9}
	\myvec{1 & 0\\0 & 1\\\frac{1}{2} & \frac{1}{3}} \myvec{\alpha_1 \\ \alpha_2} &=\myvec{-2\\\frac{5}{2}\\-4}\\\label{eq:solutions/4/44/1/d/eq10}
	\vec{M}\vec{x} &= \vec{b}\label{eq:solutions/4/44/1/d/eq11}
\intertext{Where,}
    \vec{M} &= \myvec{1 & 0\\0 & 1\\\frac{1}{2} & \frac{1}{3}} \\
    \vec{x} &= \myvec{\alpha_1 \\ \alpha_2} \\
    \vec{b} &= \myvec{-2\\\frac{5}{2}\\-4}
\end{align}
Applying Singular Value Decomposition on $\vec{M}$,
\begin{align} \label{eq:solutions/4/44/1/d/eq:eq_6}
    \vec{M}=\vec{U}\vec{S}\vec{V}^T
\end{align}
Where the columns of $\vec{V}$ are the eigenvectors of $\vec{M}^T\vec{M}$, the columns of $\vec{U}$ are the eigenvectors of $\vec{M}\vec{M}^T$ and $\vec{S}$ is diagonal matrix of singular values of $\vec{M}^T\vec{M}$.
\begin{align}
    \vec{M}^T \vec{M} &= \myvec{\tfrac{5}{4} & \tfrac{1}{6}  \\\tfrac{1}{6}  & \tfrac{10}{9} }\label{eq:solutions/4/44/1/d/eq:eq_7} \\
    \vec{M} \vec{M}^T &= \myvec{1 & 0 & \frac{1}{2}\\ 0 & 1 & \frac{1}{3} \\ \tfrac{1}{2} & \tfrac{1}{3} & \tfrac{13}{36}} \label{eq:solutions/4/44/1/d/eq:eq_8}
\end{align}
From \eqref{eq:solutions/4/44/1/d/eq11} and \eqref{eq:solutions/4/44/1/d/eq:eq_6},
\begin{align}
    \vec{U} \vec{S} \vec{V}^T \vec{x} = \vec{b} \nonumber \\
    \implies \vec{x} = \vec{V} \vec{S_+} \vec{U^T} \vec{b} \label{eq:solutions/4/44/1/d/eq:eq_9}
\end{align}
Where $\vec{S_+}$ is Moore-Penrose Pseudo-Inverse of $\vec{S}$. Calculating eigenvalues of $\vec{M}\vec{M}^T$,
\begin{align}
    \mydet{\vec{M} \vec{M}^T - \lambda \vec{I}} = 0 \nonumber \\
    \implies \mydet{1-\lambda & 0 & \frac{1}{2} \\ 0 & 1-\lambda & \frac{1}{3} \\ \frac{1}{2} & \frac{1}{3} & \frac{13}{36}-\lambda} &= 0 \nonumber \\
    \implies \lambda^3 - \frac{85}{36}\lambda^2 + \frac{49}{36}\lambda =0 \nonumber
\end{align}
Hence eigenvalues of $\vec{M}\vec{M}^T$ are,
\begin{align} \label{eq:solutions/4/44/1/d/eq:eq_10}
    \lambda_1 = \frac{49}{36}; \quad \lambda_2 = 1; \quad \lambda_3 =0
\end{align}
And the corresponding eigenvectors are,
\begin{align}
     \vec{u_1} = \myvec{18 \\12 \\ 13}; \quad \vec{u_2} = \myvec{-2 \\3 \\ 0};\quad 
    \vec{u_3} = \myvec{-3 \\ -2 \\ 6}\label{eq:solutions/4/44/1/d/eq:eq_11} 
\end{align}
Normalizing the above eigenvectors,
\begin{align} 
     \vec{u_1} = \myvec{\tfrac{18}{7\sqrt{13}} \\\tfrac{12}{7\sqrt{13}}\\ \tfrac{13}{7\sqrt{13}}}; \quad 
    \vec{u_2} = \myvec{\frac{-2}{\sqrt{13}} \\\frac{3}{\sqrt{13}} \\ 0}; \quad 
    \vec{u_3} = \myvec{\tfrac{-3}{7} \\ \tfrac{-2}{7} \\ \tfrac{6}{7}}
  \label{eq:solutions/4/44/1/d/eq:eq_12}
\end{align}
From \eqref{eq:solutions/4/44/1/d/eq:eq_12} we obtain $\vec{U}$ as,
\begin{align} \label{eq:solutions/4/44/1/d/eq:eq_13}
    \vec{U} = \myvec{\tfrac{18}{7\sqrt{13}} & \frac{-2}{\sqrt{13}} &\tfrac{-3}{7} \\ \tfrac{12}{7\sqrt{13}} & \frac{3}{\sqrt{13}} & \tfrac{-2}{7}  \\  \tfrac{13}{7\sqrt{13}} & 0 & \tfrac{6}{7}}
\end{align}
Using values from \eqref{eq:solutions/4/44/1/d/eq:eq_10},
\begin{align} \label{eq:solutions/4/44/1/d/eq:eq_14}
    \vec{S} = \myvec{\frac{7}{6} & 0 \\ 0 & 1 \\ 0 & 0} 
\end{align}
Calculating the eigenvalues of $\vec{M}^T\vec{M}$,
\begin{align}
    \mydet{\vec{M}^T\vec{M} - \lambda \vec{I}} = 0 \nonumber \\
    \implies \mydet{\tfrac{5}{4}-\lambda & \frac{1}{6} \\ \frac{1}{6} & \tfrac{10}{9}-\lambda} &= 0 \nonumber \\
    \implies \lambda^2 - \frac{85}{36}\lambda + \frac{49}{36} =0 \nonumber
\end{align}
Hence, eigenvalues of $\vec{M}^T\vec{M}$ are,
\begin{align}
    \lambda_4 = \frac{49}{36}; \quad \lambda_5 = 1 \nonumber
\end{align}
And the corresponding eigenvectors are,
\begin{align}
    \vec{v_1} = \myvec{3 \\2 }; \quad \vec{v_2} = \myvec{-2 \\3};\nonumber
    \intertext{Normalizing the above eigenvectors,}
     \vec{v_1} = \myvec{\frac{3}{\sqrt{13}}  \\ \frac{2}{\sqrt{13}}}; \quad 
    \vec{v_2} = \myvec{\frac{-2}{\sqrt{13}}\\\frac{3}{\sqrt{13}}} \label{eq:solutions/4/44/1/d/eq:eq_15}
\end{align}
From\eqref{eq:solutions/4/44/1/d/eq:eq_15} we obtain $\vec{V}$ as,
\begin{align} \label{eq:solutions/4/44/1/d/eq:eq_16}
    \vec{V} = \myvec{\frac{3}{\sqrt{13}} & \frac{-2}{\sqrt{13}}\\ \frac{2}{\sqrt{13}} & \frac{3}{\sqrt{13}}}
\end{align}
From \eqref{eq:solutions/4/44/1/d/eq:eq_6} we get the Singular Value Decomposition of $\vec{M}$,
\begin{align} \label{eq:solutions/4/44/1/d/eq:eq_17}
    \vec{M} =  \myvec{\tfrac{18}{7\sqrt{13}} & \frac{-2}{\sqrt{13}} &\tfrac{-3}{7} \\ \tfrac{12}{7\sqrt{13}} & \frac{3}{\sqrt{13}} & \tfrac{-2}{7}  \\  \tfrac{13}{7\sqrt{13}} & 0 & \tfrac{6}{7}} 
    \myvec{\frac{7}{6} & 0 \\ 0 & 1 \\ 0 & 0}  \myvec{\frac{3}{\sqrt{13}} & \frac{-2}{\sqrt{13}}\\ \frac{2}{\sqrt{13}} & \frac{3}{\sqrt{13}}}
\end{align}
Moore-Penrose Pseudo inverse of $\vec{S}$ is given by,
\begin{align} \label{eq:solutions/4/44/1/d/eq:eq_18}
    \vec{S_+} =\myvec{\frac{6}{7} & 0 & 0 \\ 0 & 1 &0 }
\end{align}
From \eqref{eq:solutions/4/44/1/d/eq:eq_9},
\begin{align}
    \vec{U}^T\vec{b} &= \myvec{\tfrac{-58}{7\sqrt{13}} \\ 
    \tfrac{23}{2\sqrt{13}} \\ \tfrac{-23}{7}} \nonumber \\
    \vec{S_+}\vec{U}^T\vec{d} &= \myvec{\frac{-348}{49\sqrt{13}} \\ \frac{23}{2\sqrt{13}}} \nonumber \\
    \vec{x} = \vec{V}\vec{S_+}\vec{U}^T\vec{d} &= \boxed{\myvec{\frac{-167}{49} \\ \frac{153}{98}}} \label{eq:solutions/4/44/1/d/eq:eq_19}
\end{align}
To verify the value of $\vec{x}$ obtained from \eqref{eq:solutions/4/44/1/d/eq:eq_19},
\begin{align} \label{eq:solutions/4/44/1/d/eq:eq_20}
    \vec{M}^T\vec{M}\vec{x} = \vec{M}^T\vec{b}
\end{align}
Substituting the values from \eqref{eq:solutions/4/44/1/d/eq:eq_7} in \eqref{eq:solutions/4/44/1/d/eq:eq_20},
\begin{align}
    \myvec{\frac{5}{4} & \frac{1}{6} \\\frac{1}{6} & \frac{10}{9}}\vec{x} = \myvec{-4 \\ \frac{7}{6}} \nonumber
\end{align}
Converting the above equation into augmented form and solving for $\vec{x}$,
\begin{align}
    \myvec{\frac{5}{4} & \frac{1}{6} & -4\\ \frac{1}{6} & \frac{10}{9} &\frac{7}{6}}\nonumber\\ 
    \xleftrightarrow[]{R_1 \leftarrow \frac{4}{5}R_1} 
    \myvec{1 & \frac{2}{15} & \frac{-16}{5} \\ \frac{1}{6} & \frac{10}{9} & \frac{7}{6}} \nonumber \\ 
    \xleftrightarrow[]{R_2 \leftarrow R_2-\frac{1}{6}R_1} \myvec{1 & \frac{2}{15} & \frac{-12}{5} \\ 0 & \frac{49}{45} & \frac{17}{10}}\nonumber\\
    \xleftrightarrow[]{R_2 \leftarrow \frac{45}{49}R_2} \myvec{1 & \frac{2}{15} & \frac{-12}{5} \\ 0 & 1 & \frac{153}{98}}\nonumber\\
    \xleftrightarrow[]{R_1 \leftarrow R_1-\frac{2}{15}R_2} \myvec{1 & 0 & \frac{-167}{49} \\ 0 & 1 & \frac{153}{98}}\label{eq:solutions/4/44/1/d/eq:eq_22}
\end{align}
From \eqref{eq:solutions/4/44/1/d/eq:eq_22} it can be observed that,
\begin{align} 
    \vec{x} = \myvec{\frac{-167}{49} \\ \frac{153}{98}} 
\end{align}
Hence verified.\\
Thus, the point $\vec{Q}$ (foot of the perpendicular) can be obtained by putting values of $\alpha_1$ and $\alpha_2$ in \eqref{eq:solutions/4/44/1/d/eq_25}:
\begin{align}
    \vec{Q} = \myvec{1\\\frac{-1}{2}\\0} + \frac{-167}{49}\myvec{1\\0\\\frac{1}{2}} +  \frac{153}{98}\myvec{0\\1\\\frac{1}{3}}\\
    \boxed{\vec{Q} = \myvec{\tfrac{-118}{49}\\\tfrac{52}{49}\\\tfrac{-58}{49}}}
\end{align}
The distance between the point $D$ and the plane can be obtained as:
\begin{align}
    \norm{\vec{Q}-\vec{d}}=\sqrt{\brak{\tfrac{-118}{49}+1}^2+\brak{\tfrac{52}{49}-2}^2+\brak{\tfrac{-58}{49}+4}^2}\\
    \boxed{\norm{\vec{Q}-\vec{d}}=\frac{23}{7}=3.2857} \label{eq:solutions/4/44/1/d/eq_54}
\end{align}
Thus the distance obtained in equation \eqref{eq:solutions/4/44/1/d/eq_20} by projection method is matches with the distance obtained in equation \eqref{eq:solutions/4/44/1/d/eq_54}. Hence verified.
