%The above equation can be expressed in the form 
%\vec{x}^T\vec{V}\vec{x}+2\vec{u}^T\vec{x}+f&=0
%%\label{eq:solutions/40/7/2.2} 
%\label{eq:solutions/40/7/eq1}
\begin{enumerate}
\item  \eqref{eq:hyper_asymp} can be expressed as \eqref{eq:conic_quad_form} with 
\begin{align}
    \vec{V}=\vec{V}^T&=\myvec{8 & 5 \\ 5 &-3}\label{eq:solutions/40/7/eqv}\\
    \vec{u}&=\myvec{-1 \\2 }\label{eq:solutions/40/7/equ}\\
    f&=-2\label{eq:solutions/40/7/eqfv}
\end{align}   
Expanding the Determinant of $\vec{V}$,
\begin{align}
    \Delta_{V} &= \mydet
%\begin{array}{|cc|}
{
8 &5
\\
5 & -3
}
= -49 < 0
%\end{array}<0
\label{eq:solutions/40/7/eq:hyp}
\end{align}
Hence from \eqref{eq:conic_hyper_cond} and \eqref{eq:solutions/40/7/eq:hyp}, \eqref{eq:hyper_asymp}
%\eqref{eq:solutions/40/7/eq:hyp} 
represents a hyperbola.
The characteristic equation of $\vec{V}$ is obtained by evaluating the determinant 
\begin{align}
%       \begin{array}{|c|}
\mydet{V-\lambda\vec{I}} = 0
\\
%\end{array}&=0\\
%   \begin{array}{|cc|}
\mydet{
8-\lambda & 5 \\ 5 & -3-\lambda
} = 0
\\
%\end{array}&=0\\
    \brak{8-\lambda}\brak{-3-\lambda}-25=0\\
    \lambda_{1}= \frac{5+\sqrt{221}}{2}\label{eq:solutions/40/7/eq:matrix_l1}\\
    \lambda_{2}= \frac{5-\sqrt{221}}{2}\label{eq:solutions/40/7/eq:matrix_l2}
\end{align}
The eigenvector $\vec{p}$ is defined as 
\begin{align}
    \vec{V}\vec{p}&=\lambda\vec{p}\\
    \implies (\vec{V}-\lambda\vec{I})\vec{p}&=0\label{eq:solutions/40/7/eq:7/eqev}
\end{align}
For $\lambda_1=\frac{5+\sqrt{221}}{2}$ ,
\begin{align}
    (\vec{V}-\lambda_1\vec{I})=\myvec{\frac{11-\sqrt{221}}{2} & 5 \\5 & \frac{-11-\sqrt{221}}{2}}
\end{align}
By row reduction, 
\begin{align}
    &\myvec{\frac{11-\sqrt{221}}{2} & 5 \\5 & \frac{-11-\sqrt{221}}{2}}\\
    %&\xleftrightarrow{\frac{R_1}{\frac{\sqrt{533}+2}{2}}}\\
    &\xleftrightarrow{R_1\leftarrow R_2}
    \myvec{\frac{-11-\sqrt{221}}{2} & 5 \\ \frac{11-\sqrt{221}}{2} & 5}\\
 &\xleftrightarrow{R_2\leftarrow R_2-\frac{11-\sqrt{221}}{10}R_{1}}
    \myvec{5 & \frac{-11-\sqrt{221}}{2} \\ 0& 0}\\
     &\xleftrightarrow{R_1\leftarrow R_1/5}
    \myvec{1 & \frac{-11-\sqrt{221}}{10} \\ 0& 0}
    \label{eq:solutions/40/7/eq:7/eqs1}
\end{align}
Substituting \eqref{eq:solutions/40/7/eq:7/eqs1} in \eqref{eq:solutions/40/7/eq:7/eqev} we get
\begin{align}
        & \myvec{1 & \frac{-11-\sqrt{221}}{10} \\ 0& 0}\myvec{v_1 \\ v_2}=\myvec{0 \\ 0}\label{eq:solutions/40/7/eq:7/eqei1}
\end{align}
Where, $\vec{p}=\myvec{v_1\\v_2}$
Let $v_2=t$
\begin{align}
    v_1&=\frac{t(11+\sqrt{221})}{10}
\end{align}
Eigen vector $\vec{p_1}$ is given by
\begin{align}
    \vec{p_1}&=\myvec{\frac{t(11+\sqrt{221})}{10} \\ t}
\end{align}
Let $t=1$, we get
\begin{align}
        \vec{p_1}&=\myvec{\frac{11+\sqrt{221}}{10} \\1 }\label{eq:solutions/40/7/eq:es71/eqp1}
\end{align}
For $\lambda_2=\frac{5-\sqrt{221}}{2}$ ,
\begin{align}
    (\vec{V}-\lambda_2\vec{I})=\myvec{\frac{11+\sqrt{221}}{2} & 5 \\5 & \frac{-11+\sqrt{221}}{2}}
\end{align}
By row reduction , 
\begin{align}
     \myvec{\frac{11+\sqrt{221}}{2} & 5 \\5 & \frac{-11+\sqrt{221}}{2}}
\\
    \xleftrightarrow{R_1\leftarrow R_2+ \frac{11-\sqrt{221}}{10}R_1}
     \myvec{\frac{11+\sqrt{221}}{2} &5\\ 0& 0}\\  
 \xleftrightarrow{R_1\leftarrow
 \frac{R_1}{\frac{11+\sqrt{221}}{10}}}
    \myvec{1 & \frac{10}{11+\sqrt{221}} \\ 0& 0}
    \label{eq:solutions/40/7/eq:es71/eqs2}
\end{align} 
Substiuting \eqref{eq:solutions/40/7/eq:es71/eqs2} in \eqref{eq:solutions/40/7/eq:7/eqev} we get 
\begin{align}
    &\myvec{1 & \frac{10}{11+\sqrt{221}} \\0 & 0}\myvec{v_1 \\ v_2}=\myvec{0 \\ 0}
%\label{eq:solutions/40/7/eq:es71/eqei1}
\end{align}
Where, $\vec{p}=\myvec{v_1\\v_2}$
Let $v_2=t$
\begin{align}
    v_1&=\frac{-t\brak{10}}{11+\sqrt{221}}
\end{align}
Eigen vector $\vec{p_2}$ is given by
\begin{align}
        \vec{p_2}&=\myvec{\frac{-t\brak{10}}{11+\sqrt{221}} \\ t}
\end{align}
Let $t=1$, we get 
\begin{align}
    \vec{p_2}&=\myvec{\frac{\brak{-10}}{11+\sqrt{221}} \\1 }\label{eq:solutions/40/7/eq:es71/eqp2}
\end{align}
By eigen decompostion $\vec{V}$ can be represented by
\begin{align}
    \vec{V}&=\vec{P}\vec{D}\vec{P}^T\label{eq:solutions/40/7/eq:es71/eqsubs}
\end{align}
where 
\begin{align}
        \vec{P}&=\myvec{\vec{p_1} & \vec{p_2}}\label{eq:solutions/40/7/eq:es71/eqp}\\
    \vec{D}&=\myvec{\lambda_1 & 0 \\0 & \lambda_2}\label{eq:solutions/40/7/eq:es71/eqD}
\end{align}
Substituting equations \ref{eq:solutions/40/7/eq:es71/eqp1}, \ref{eq:solutions/40/7/eq:es71/eqp2} in \eqref{eq:solutions/40/7/eq:es71/eqp} we get 
\begin{align}
    \vec{P}&=\myvec{\frac{11+\sqrt{221}}{10} & \frac{-10}{11+\sqrt{221}} \\1 & 1}\label{eq:solutions/40/7/eq:es71/eqP}
\end{align}
Substituting equations \ref{eq:solutions/40/7/eq:matrix_l1}, \ref{eq:solutions/40/7/eq:matrix_l2} in \ref{eq:solutions/40/7/eq:es71/eqD} we get
\begin{align}
       \vec{D}&=\myvec{\frac{5+\sqrt{221}}{2} & 0\\0 & \frac{5-\sqrt{221}}{2}}\label{eq:solutions/40/7/eq:es71/eqDD}
\end{align}
Centre of the hyperbola is given by 
\begin{align}
    \vec{c}&=-\vec{V}^{-1}\vec{u}\\
    \implies\vec{c}&=-\myvec{\frac{3}{49}&\frac{5}{49}\\\frac{5}{49}&\frac{-8}{49}}\myvec{-1 \\ 2}\\
    \implies\vec{c}&=\myvec{\frac{-3}{49}&\frac{-5}{49}\\\frac{-5}{49}&\frac{8}{49}}\myvec{-1 \\ 2}\\
    \implies\vec{c}&=\myvec{\frac{-1}{7}\\\frac{3}{7}}
\end{align}
Since,
\begin{align}
    \vec{u}^T\vec{V}^{-1}\vec{u}-f = 1 > 0\label{eq:solutions/40/7/eq:es71/cond}
\end{align} 
there isn't a need to swap axes
In hyperbola,
\begin{align}
axes=
\begin{cases}
\sqrt{\frac{\vec{u}^T\vec{V}^{-1}\vec{u}-f}{\lambda_1}}\\ \sqrt{\frac{f-\vec{u}^T\vec{V}^{-1}\vec{u}}{\lambda_2}}
\end{cases}
\end{align}
From above equations we can say that,
\begin{align}
\sqrt{\frac{\vec{u}^T\vec{V}^{-1}\vec{u}-f}{\lambda_1}}=\sqrt{ \frac{2}{5+\sqrt{221}}}\\
\sqrt{\frac{f-\vec{u}^T\vec{V}^{-1}\vec{u}}{\lambda_2}}=\sqrt{ \frac{2}{5-\sqrt{221}}}
\end{align}
The equation of the hyperbola at the origin is then given by \eqref{eq:conic_simp_temp_nonparab} as
 %Now we have,
\begin{align}
    \vec{y}^T\vec{D}\vec{y}&=\vec{u}^T\vec{V}^{-1}\vec{u}-f\label{eq:solutions/40/7/eq:es71/fi}
%\end{align}
%where ,
%\begin{align}
%    \vec{y}&=\vec{P}^T(\vec{x}-\vec{c})
%\end{align}
%To get $\vec{y}$,
%\begin{align}
%\vec{y}&=\vec{P}^T\vec{x}-\vec{P}^T\vec{c}\\
%    \vec{y}&= \myvec{\frac{11+\sqrt{221}}{10} & 1 \\ \frac{-10}{11+\sqrt{221}} & 1}\vec{x}-\myvec{\frac{11+\sqrt{221}}{10} & 1 \\ \frac{-10}{11+\sqrt{221}} & 1}\myvec{\frac{-1}{7}\\\frac{3}{7}}\\
%    \vec{y}&=\myvec{\frac{11+\sqrt{221}}{10} & 1 \\ \frac{-10}{11+\sqrt{221}} & 1}\vec{x}-\myvec{\frac{-11-\sqrt{221}}{70}+\frac{3}{7} \\ \frac{10}{(7)11+(7)\sqrt{221}}+\frac{3}{7}}
%\end{align}
%substituting the eqauations \eqref{eq:solutions/40/7/eq:es71/cond}, \eqref{eq:solutions/40/7/eq:es71/eqDD} in equation \eqref{eq:solutions/40/7/eq:es71/fi}
%\begin{align}
\\
   \implies\vec{y}^T\myvec{\frac{5+\sqrt{221}}{2} & 0 \\0 & \frac{5-\sqrt{221}}{2}}\vec{y}&= 1
\end{align}
\item ({\em Asymptotes of hyperbola: })
The equation for the asymptotes of \eqref{eq:hyper_asymp} is given by \eqref{eq:asymp_quad_form} with 

%Equation of a hyperbola and the combined equation of the Asymptotes differ only in the constant term.
%\begin{align}
% 8x^2+10xy-3y^2-2x+4y+K=0   
%\end{align}
%The above equation can be expressed in the form 
%\begin{align}
%\vec{x}^T\vec{V}\vec{x}+2\vec{u}^T\vec{x}+f&=0
%\label{eq:solutions/40/7/2.2} 
%\label{eq:solutions/40/7/eq1}
%\intertext{Comparing equation we get}
%    \vec{V}=\vec{V}^T&=\myvec{8 & 5 \\ 5 &-3}\label{eq:solutions/40/7/es1/eqv}\\
%    \vec{u}&=\myvec{-1 \\2 }\label{eq:solutions/40/7/eq:equ}\\
%    f&=K\label{eq:solutions/40/7/eq:es1/eqfv}
%\end{align}   
\begin{align}
\Delta&=
%\begin{array}{|ccc|}
\mydet{
8 & 5 & -1\\ 5& -3 & 2\\ -1 & 2 & K
} = 0
%\end{array}
\\
\implies K&=-1
\end{align}
using \eqref{eq:quad_form_asymp_cond}.  From \eqref{eq:quad_pair_slopes},  \eqref{eq:hyper_asymp} and \eqref{eq:quad_pair_norm_vec},
%Similar way expanding the Determinant of $\vec{V}$.
%\begin{align}
%    \Delta_{V} &= \begin{array}{|cc|}
%8 &5\\5 & -3
%\end{array}<0\label{eq:solutions/40/7/eq:es/17/hyp}
%\end{align}
%From \eqref{eq:solutions/40/7/eq:es/17/hyp} we could say that the given equation represents two straight lines
%Let the equations of lines be,
%\begin{align}
%	\brak{\vec{n_1}^T \vec{x} - c_1}\brak{\vec{n_1}^T \vec{x} - c_1} =
%        \vec{x}^{T}\vec{Vx} + 2\vec{u}^{T}\vec{x} + f=0\label{eq:solutions/40/7/eq:eql7/03}
%\end{align}
%\begin{align}
%\brak{\vec{n_1}^T\vec{x}-c_1}\brak{\vec{n_2}^T\vec{x}-c_2}
%&=\vec{x}^T\myvec{8 & 5 \\ 5 & -3}\vec{x}\notag\\
%+2\myvec{-1 & 2}\vec{x}-1\label{eq:solutions/40/7/equate}\\
%    \vec{n_1}*\vec{n_2} = \myvec{a\\2b\\c} &= \myvec{8\\10\\-3}\label{eq:solutions/40/7/conv}\\
%    c_2\vec{n_1}+c_1\vec{n_2}&=-2\myvec{-1\\2}\label{eq:solutions/40/7/eq17/c1c2}\\
%    c_1c_2&=-1
%\end{align}
%The slopes of the lines are given by the roots of the polynomial 
%\begin{align}
%    &cm^2+2bm+a=0\label{eq:solutions/40/7/e}\\
%    \implies m_i&=\frac{-b\pm{\sqrt{-\Delta_{V}}}}{c}\\
%    \vec{n_i}&=k\myvec{-m_i\\1}
%\end{align}
%Substituting the given data in above equations \eqref{eq:solutions/40/7/e} we get,
\begin{align}
    -3m^2+10m+8&=0\\
    m_1=4,  m_2&=\frac{-2}{3}\\
   \implies  \vec{n_1}=\myvec{-4\\ 1}, \vec{n_2}&=\myvec{-2\\-3} \label{eq:solutions/40/7/eq:normal1}
%\intertext{We know that,}
%& \vec{n_1}\ast \vec{n_2} = \myvec{a\\2b\\c} \label{eq:solutions/40/7/eq:conv1}
\end{align}
%
%Verification using Toeplitz matrix, 
From equation \eqref{eq:solutions/40/7/eq:normal1},
the Toeplitz matrix for $\vec{n}_1$ is
\begin{align}
    T_{\vec{n_1}}=\myvec{-4&0\\1&-4\\0&-1}
\end{align}
The product of the above matrix with $\vec{n_2}$ is
\begin{align}
T_{\vec{n_1}}    \vec{n_2}=
%\myvec{-2\\-3}\label{eq:solutions/40/7/eq:conv2}\\
%\implies 
\myvec{-4&0\\1&-4\\0&1}\myvec{0\\ -1} = \myvec{8\\10\\-3}  =\myvec{a\\2b\\c}\label{eq:solutions/40/7/eq:conv3}
\end{align}
in \eqref{eq:hyper_asymp} and is equivalent to the convolution operation in \eqref{eq:quad_pair_conv},
providing a verification of \eqref{eq:solutions/40/7/eq:normal1}.
%which 
%$\implies$ Equation \eqref{eq:solutions/40/7/eq:normal1} satisfies \eqref{eq:solutions/40/7/eq:conv1}\\
%$c_1$ and $c_2$ can be obtained 
From \eqref{eq:quad_pair_ci_mat}
\begin{align}
\myvec{\vec{n_1} & \vec{n_2}}\myvec{c_2\\c_1}&=-2\vec{u} \label{eq:solutions/40/7/eq:aug1}
\end{align}
Substituting \eqref{eq:solutions/40/7/eq:normal1} in \eqref{eq:solutions/40/7/eq:aug1}, the augmented matrix is,
\begin{align}
\myvec{-4 & -2 & -2 \\ 1 & -3 & 4}
\xleftrightarrow[R_2\leftarrow R_2-R_1]{R_1\leftarrow -R_1/4}
\myvec{1 &\frac{1}{2} &\frac{1}{2} \\ 0 & -\frac{7}{2} & \frac{7}{2}} \label{eq:solutions/40/7/eq:aug5}\\
\xleftrightarrow[R_1\leftarrow R_1-\frac{1}{2}R_2]{R_2\leftarrow -\frac{2}{7}R_2}
\myvec{1 &0 &1 \\ 0& 1 & -1} \label{eq:solutions/40/7/eq:aug2}\\
\implies c_1 = 1, c_2=-1 \label{eq:solutions/40/7/eq:const1}
\end{align}
Thus, from \eqref{eq:solutions/40/7/eq:normal1} and \eqref{eq:solutions/40/7/eq:const1}, the desired equations of the asymptotes are 
%Equations \eqref{eq:solutions/40/7/eq:eql7/03}, can be modified as,from \eqref{eq:solutions/40/7/eq:normal1} and \eqref{eq:solutions/40/7/eq:const1} in we get,
\begin{align}
    \myvec{-4 & 1}\vec{x}&=1\\
    \myvec{-2 & -3}\vec{x}&=-1
\end{align}
%\begin{multline}
%\implies \brak{-4x+y-1}\brak{-2x-3y+1}= 0\\
%\implies \boxed{\brak{4x-y+1}\brak{2x+3y-1} = 0} \label{eq:solutions/40/7/eq:line1}
%\end{multline}
The angle between the lines can be expressed as, 
\begin{align}
	\vec{n_1}=\myvec{-4\\1} , \quad \vec{n_2}=\myvec{-2\\-3}\\
	\cos\theta=\frac{\vec{n_1}^T\vec{n_2}}{\norm{\vec{n_1}}\norm{\vec{n_2}}} \\
	\implies \quad \theta=\cos^{-1}\brak{\frac{5}{\sqrt{221}}}.
\end{align}
\item {Conjugate Hyperbola: }  The conjugate hyperbola is obtained from \eqref{eq:hyper_asymp} and  \eqref{eq:conic_quad_form}
as 
\begin{align}
\label{eq:conic_quad_form_conjugate}
\vec{x}^T\vec{V}\vec{x}+2\vec{u}^T\vec{Q}\vec{x}+f=0
\end{align}
%
where 
\begin{align}
\vec{Q} = \myvec{
\cos \theta & -\sin \theta
\\
\sin \theta & \cos \theta 
} 
\end{align}
is a rotation matrix and $\theta$ is the angle between the asymptotes.
%The characteristic equation of $\vec{V}$ is obtained by evaluating the determinant \eqref{eq:solutions/40/7/es1/eqv}
%\begin{align}
%       \begin{array}{|c|}
%V-\lambda\vec{I}
%\end{array}&=0\\
%   \begin{array}{|cc|}
%8-\lambda & 5 \\ 5 & -3-\lambda
%\end{array}&=0\\
%    \brak{8-\lambda}\brak{-3-\lambda}-25=0\\
%    \lambda_{1}= \frac{5+\sqrt{221}}{2}\\
%    \lambda_{2}= \frac{5-\sqrt{221}}{2}
%\end{align}
%The eigenvector $\vec{p}$ is defined as 
%\begin{align}
%    \vec{V}\vec{p}&=\lambda\vec{p}\\
%    \implies (\vec{V}-\lambda\vec{I})\vec{p}&=0\label{eq:solutions/40/7/eq:es/2701}
%\end{align}
%For $\lambda_1=\frac{5+\sqrt{221}}{2}$ ,
%\begin{align}
%    (\vec{V}-\lambda_1\vec{I})=\myvec{\frac{11-\sqrt{221}}{2} & 5 \\5 & \frac{-11-\sqrt{221}}{2}}
%\end{align}
%By row reduction , 
%\begin{align}
%    &\myvec{\frac{11-\sqrt{221}}{2} & 5 \\5 & \frac{-11-\sqrt{221}}{2}}\\
%    %&\xleftrightarrow{\frac{R_1}{\frac{\sqrt{533}+2}{2}}}\\
%    &\xleftrightarrow{R_1\leftarrow R_2}
%    \myvec{\frac{-11-\sqrt{221}}{2} & 5 \\ \frac{11-\sqrt{221}}{2} & 5}\\
% &\xleftrightarrow{R_2\leftarrow R_2-\frac{11-\sqrt{221}}{10}R_{1}}
%    \myvec{5 & \frac{-11-\sqrt{221}}{2} \\ 0& 0}\\
%     &\xleftrightarrow{R_1\leftarrow R_1/5}
%    \myvec{1 & \frac{-11-\sqrt{221}}{10} \\ 0& 0}
%    \label{eq:solutions/40/7/eq:es27/02}
%\end{align}
%substituting \eqref{eq:solutions/40/7/eq:es27/02} in \eqref{eq:solutions/40/7/eq:es/2701} we get
%\begin{align}
%        & \myvec{1 & \frac{-11-\sqrt{221}}{10} \\ 0& 0}\myvec{v_1 \\ v_2}=\myvec{0 \\ 0}\label{eq:solutions/40/7/eq:es27/eqei1}
%\end{align}
%Where, $\vec{p}=\myvec{v_1\\v_2}$
%Let $v_2=t$
%\begin{align}
%    v_1&=\frac{t(11+\sqrt{221})}{10}
%\end{align}
%Eigen vector $\vec{p_1}$ is given by
%\begin{align}
%    \vec{p_1}&=\myvec{\frac{t(11+\sqrt{221})}{10} \\ t}
%\end{align}
%Let $t=1$, we get
%\begin{align}
%        \vec{p_1}&=\myvec{\frac{11+\sqrt{221}}{10} \\1 }\label{eq:solutions/40/7/eq:es27/eqp1}
%\end{align}
%For $\lambda_2=\frac{5-\sqrt{221}}{2}$ ,
%\begin{align}
%    (\vec{V}-\lambda_2\vec{I})=\myvec{\frac{11+\sqrt{221}}{2} & 5 \\5 & \frac{-11+\sqrt{221}}{2}}
%\end{align}
%By row reduction, 
%\begin{align}
%    \myvec{\frac{11+\sqrt{221}}{2} & 5 \\5 & \frac{-11+\sqrt{221}}{2}}
%\\
%    \xleftrightarrow{R_1\leftarrow R_2+ \frac{11-\sqrt{221}}{10}R_1}
%     \myvec{\frac{11+\sqrt{221}}{2} &5\\ 0& 0}\\  
% \xleftrightarrow{R_1\leftarrow
% \frac{R_1}{\frac{11+\sqrt{221}}{10}}}
%    \myvec{1 & \frac{10}{11+\sqrt{221}} \\ 0& 0}
%    \label{eq:solutions/40/7/eq:es27eqs02}
%\end{align}
%substituting \eqref{eq:solutions/40/7/eq:es27eqs02} in \eqref{eq:solutions/40/7/eq:es/2701} we get 
%\begin{align}
%    &\myvec{1 & \frac{10}{11+\sqrt{221}} \\0 & 0}\myvec{v_1 \\ v_2}=\myvec{0 \\ 0}
%%\label{eq:solutions/40/7/eq:es27/eqei1}
%\end{align}
%Where, $\vec{p}=\myvec{v_1\\v_2}$
%Let $v_2=t$
%\begin{align}
%    v_1&=\frac{-t\brak{10}}{11+\sqrt{221}}
%\end{align}
%Eigen vector $\vec{p_2}$ is given by
%\begin{align}
%        \vec{p_2}&=\myvec{\frac{-t\brak{10}}{11+\sqrt{221}} \\ t}
%\end{align}
%Let $t=1$, we get 
%\begin{align}
%    \vec{p_2}&=\myvec{\frac{\brak{-10}}{11+\sqrt{221}} \\1 }\label{eq:solutions/40/7/eq:es27/eqp2}
%\end{align}
%By eigen decompostion $\vec{V}$ can be represented by
%\begin{align}
%    \vec{V}&=\vec{P}\vec{D}\vec{P}^T\label{eq:solutions/40/7/eq:es27/eqsubs}
%\end{align}
%where 
%\begin{align}
%        \vec{P}&=\myvec{\vec{p_1} & \vec{p_2}}\label{eq:solutions/40/7/eq:es27/eqp}\\
%    \vec{D}&=\myvec{\lambda_1 & 0 \\0 & \lambda_2}\label{eq:solutions/40/7/eq:es27/eqD}
%\end{align}
%Substituting equations \ref{eq:solutions/40/7/eq:es27/eqp1}, \ref{eq:solutions/40/7/eq:es27/eqp2} in \eqref{eq:solutions/40/7/eq:es27/eqp} we get 
%\begin{align}
%    \vec{P}&=\myvec{\frac{11+\sqrt{221}}{10} & \frac{-10}{11+\sqrt{221}} \\1 & 1}\label{eq:solutions/40/7/eq:es27/eqP}
%\end{align}
%\begin{align}
%       \vec{D}&=\myvec{\frac{5+\sqrt{221}}{2} & 0\\0 & \frac{5-\sqrt{221}}{2}}\label{eq:solutions/40/7/eq:es27/eqDD}
%\end{align}
%Centre of the hyperbola is given by 
%\begin{align}
%    \vec{c}&=-\vec{V}^{-1}\vec{u}\\
%    \implies\vec{c}&=-\myvec{\frac{3}{49}&\frac{5}{49}\\\frac{5}{49}&\frac{-8}{49}}\myvec{-1 \\ 2}\\
%    \implies\vec{c}&=\myvec{\frac{-3}{49}&\frac{-5}{49}\\\frac{-5}{49}&\frac{8}{49}}\myvec{-1 \\ 2}\\
%    \implies\vec{c}&=\myvec{\frac{-1}{7}\\\frac{3}{7}}
%\end{align}
%Since,
%\begin{align}
%    \vec{u}^T\vec{V}^{-1}\vec{u}-f = 0\label{eq:solutions/40/7/eq:es27/cond}
%\end{align} 
%Now,
%\begin{align}
%    \vec{y}^T\vec{D}\vec{y}&=\vec{u}^T\vec{V}^{-1}\vec{u}-f\label{eq:solutions/40/7/eq:es27/fi}
%\end{align}
%where ,
%\begin{align}
%    \vec{y}&=\vec{P}^T(\vec{x}-\vec{c})
%\end{align}
%To get $\vec{y}$,
%\begin{align}
%\vec{y}&=\vec{P}^T\vec{x}-\vec{P}^T\vec{c}\\
%    \vec{y}&= \myvec{\frac{11+\sqrt{221}}{10} & 1 \\ \frac{-10}{11+\sqrt{221}} & 1}\vec{x}-\myvec{\frac{11+\sqrt{221}}{10} & 1 \\ \frac{-10}{11+\sqrt{221}} & 1}\myvec{\frac{-1}{7}\\\frac{3}{7}}\\
%    \vec{y}&=\myvec{\frac{11+\sqrt{221}}{10} & 1 \\ \frac{-10}{11+\sqrt{221}} & 1}\vec{x}-\myvec{\frac{-11-\sqrt{221}}{70}+\frac{3}{7} \\ \frac{10}{(7)11+(7)\sqrt{221}}+\frac{3}{7}}
%\end{align}
%substituting the eqauations \eqref{eq:solutions/40/7/eq:es27/cond}, \eqref{eq:solutions/40/7/eq:es27/eqDD} in equation \eqref{eq:solutions/40/7/eq:es27/fi}
%Equation of asymptotes is
%\begin{align}
%    \implies \vec{y}^T\myvec{\frac{5+\sqrt{221}}{2} & 0 \\0 & \frac{5-\sqrt{221}}{2}}\vec{y}+1&=0
%\end{align}
%And the Equations of Conjugate hyperbola is 2(Equation of Asymptotes)- Equation of hyperbola. 
%\begin{align}
%    \implies \vec{y}^T\myvec{\frac{5+\sqrt{221}}{2} & 0 \\0 & \frac{5-\sqrt{221}}{2}}\vec{y}&=0
%\end{align}
\begin{figure}[h]
    \centering
    \includegraphics[width=\columnwidth]{./figs/hyper_asymp/A7_4.png}
    \caption{Hyperbola with assymptotes and its conjugate}
    \label{eq:solutions/40/7/Fig :1}
\end{figure}
\end{enumerate}
