\begin{enumerate}
\item 
\begin{align}
A = \myvec{\cos{\alpha} && \sin{\alpha} \\ $-$\sin{\alpha} && \cos{\alpha}} \\[1em]
\implies A^T = \myvec{\cos{\alpha} && $-$\sin{\alpha} \\ \sin{\alpha} && \cos{\alpha}}    
\end{align}
%Need to prove that $A^T$A = I (Identity Matrix)\\\\
%For this we express each of the matrices as a complex number to find the product of those two matrices $A^T$ and A.\\\\
%We know that a complex number \myvec{a1 \\ a2} can be represented as
\begin{align}
\myvec{a1 \\ a2} = \myvec{a1 && $-$a2 \\ a2 && a1}\myvec{1 \\ 0}\\[1em]
i.e \ A = \myvec{\cos{\alpha} \\ $-$\sin{\alpha}}\\[1em]
A^T = \myvec{\cos{\alpha} \\ \sin{\alpha}} \\[1em]
\implies A^TA = \myvec{\cos{\alpha} \\ \sin{\alpha}}\myvec{\cos{\alpha} \\ $-$\sin{\alpha}}\\[1em]
\implies A^TA = I
\end{align}\\
\item 
\begin{align}
A = \myvec{\sin{\alpha} && \cos{\alpha} \\ $-$\cos{\alpha} && \sin{\alpha}} \\[1em]
\implies A^T = \myvec{\sin{\alpha} && $-$\cos{\alpha} \\ \cos{\alpha} && \sin{\alpha}}    
\end{align}\\
%Need to prove that $A^T$A = I (Identity Matrix)\\\\
%For this we express each of the matrices as a complex number to find the product of those two matrices $A^T$ and A.\\\\
\begin{align}
i.e \ A = \myvec{\sin{\alpha} \\ $-$\cos{\alpha}}\\[1em]
A^T = \myvec{\sin{\alpha} \\ \cos{\alpha}} \\[1em]
\implies A^TA = \myvec{\sin{\alpha} \\ \cos{\alpha}}\myvec{\sin{\alpha} \\ $-$\cos{\alpha}} \\[1em]
\implies A^TA = I
\end{align}\\
%Using (3), the expressions in equation (6) and equation (12) were simplified to obtain I.\\\\
Hence Proved for both (1) and (2).
\end{enumerate}
